coq/JsCommonAux.v
@@ -62,8 +62,7 @@ Qed.
 Global Instance same_value_dec : forall v1 v2,
   Decidable (same_value v1 v2).
 Proof.
-  introv. unfold same_value. case_if. typeclass.
-  destruct (type_of v1) eqn:H1; repeat cases_if; try typeclass.
+  introv. unfold same_value. typeclass.
 Qed.
 
 Lemma if_some_bool_then_same_self : forall bo,
